examples/tactics/micro-benchmarks/UserTactics.Example1.fst
@@ -1,30 +1,30 @@
-module UserTactics.Example1 
+module UserTactics.Example1
 open FStar.Tactics
 
 #set-options "--lax"
 (* -------------------------------------------------------------------------------- *)
 let rec revert_all (bs:binders) : Tac unit =
-  match bs with 
+  match bs with
   | [] -> ()
   | _::tl -> let _ = revert () in revert_all tl
-  
-let cur_goal () : Tac goal = 
-  let goals = TAC?.get () in 
-  match goals with 
+
+let cur_goal () : Tac goal =
+  let goals = TAC?.get () in
+  match goals with
   | [], _ -> fail "No more goals"
   | hd::_, _ -> hd
 
-let destruct_equality_implication (t:term) : option (formula * term) = 
-  match term_as_formula t with 
-  | Some (Implies lhs rhs) -> 
+let destruct_equality_implication (t:term) : Tac (option (formula * term)) =
+  match term_as_formula t with
+  | Some (Implies lhs rhs) ->
     let lhs = term_as_formula lhs in
-    (match lhs with 
+    (match lhs with
      | Some (Eq _ _ _) -> Some (Some?.v lhs, rhs)
      | _ -> None)
   | _ -> None
-    
+
 let rec simplify_eq_implication : tactic unit
-  = fun () -> 
+  = fun () ->
     let context, goal_t = cur_goal () in  // G |- x=e ==> P
     match destruct_equality_implication goal_t with
     | None -> fail "Not an equality implication"
@@ -36,102 +36,102 @@ let rec simplify_eq_implication : tactic unit
 
 let rec user_visit (callback:tactic unit)
     : tactic unit
-    = fun () -> 
-         let aux : tactic unit = fun () -> 
+    = fun () ->
+         let aux : tactic unit = fun () ->
            let context, goal_t = cur_goal () in
            match term_as_formula goal_t with
            | None -> smt ()
            | Some (Exists _ _) -> //not yet handled
              ()
-             
+
            | Some (Forall xs body) ->
              let binders = forall_intros () in
              let _ = user_visit callback () in
              revert_all binders
 
-           | Some (And t1 t2) -> 
+           | Some (And t1 t2) ->
              let _ = seq split (user_visit callback) () in
              merge ()
 
-           | Some (Implies t1 t2) -> 
+           | Some (Implies t1 t2) ->
              let h = implies_intro () in
              let _ = user_visit callback () in
              revert ()
 
-           | _ -> 
+           | _ ->
              or_else trivial smt
          in
          or_else callback (user_visit callback)
 
-let rec try_rewrite_equality (x:term) 
+let rec try_rewrite_equality (x:term)
                              (bs:binders)
-  : tactic unit 
-  = fun () -> 
-    match bs with 
+  : tactic unit
+  = fun () ->
+    match bs with
     | [] -> ()
     | x_t::bs -> begin
-      match term_as_formula (type_of_binder x_t) with 
-      | Some (Eq _ y _) -> 
-        if term_eq x y 
+      match term_as_formula (type_of_binder x_t) with
+      | Some (Eq _ y _) ->
+        if term_eq x y
         then rewrite x_t
         else try_rewrite_equality x bs ()
       | _ -> try_rewrite_equality x bs ()
       end
 
 let rec rewrite_all_context_equalities (bs:binders)
-  : tactic unit 
-  = fun () -> 
-    match bs with 
+  : tactic unit
+  = fun () ->
+    match bs with
     | [] -> ()
     | x_t::bs -> begin
-      match term_as_formula (type_of_binder x_t) with 
-      | Some (Eq _ _ _) -> 
+      match term_as_formula (type_of_binder x_t) with
+      | Some (Eq _ _ _) ->
         rewrite x_t;
         rewrite_all_context_equalities bs ()
-      | _ -> 
+      | _ ->
         rewrite_all_context_equalities bs ()
       end
 
-let rec rewrite_eqs_from_context : tactic unit 
-  = fun () -> 
+let rec rewrite_eqs_from_context : tactic unit
+  = fun () ->
        let context, _ = cur_goal () in
        rewrite_all_context_equalities (binders_of_env context) ()
-       
-let rewrite_equality (x:term) : tactic unit 
-  = fun () -> 
-     let context, _ = cur_goal () in
-     try_rewrite_equality x (binders_of_env context) ()
 
-let solved : tactic unit = fun () -> 
-  let _, goal = cur_goal () in 
-  match term_as_formula goal with 
+let rewrite_equality (x:tactic term) : tactic unit
+  = fun () ->
+     let context, _ = cur_goal () in
+     try_rewrite_equality (x()) (binders_of_env context) ()
+
+let solved : tactic unit = fun () ->
+  let _, goal = cur_goal () in
+  match term_as_formula goal with
   | Some True_ -> ()
   | _ -> fail "Not solved"
 
 let rec just_do_intros : tactic unit = fun () ->
-    focus (fun () -> 
+    focus (fun () ->
        let _ = forall_intros () in
        let _ = implies_intro () in
        smt ();
        revert ();
        revert ())
 
-let rec rewrite_all_equalities : tactic unit = fun () -> 
+let rec rewrite_all_equalities : tactic unit = fun () ->
   visit simplify_eq_implication
 
 
 assume val lemma_mul_comm : x:nat -> y:nat -> Lemma (op_Multiply x y == op_Multiply y x)
 let mul_commute_ascription : tactic unit
-  = fun () -> 
+  = fun () ->
     let _, goal_t = cur_goal () in  // G |- x=e ==> P
     match term_as_formula goal_t with
     | Some (Eq _ _ _) ->
-      apply_lemma (quote lemma_mul_comm)
+      apply_lemma (quote lemma_mul_comm ())
     | _ -> fail "Not an equality"
 
-let rec unfold_definition_and_simplify_eq (tm:term) 
-  : tactic unit 
-  = fun () -> 
+let rec unfold_definition_and_simplify_eq' (tm:term)
+  : tactic unit
+  = fun () ->
       let _, goal_t = cur_goal () in  // G |- x=e ==> P
       match term_as_formula goal_t with
       | Some (App hd arg) ->
@@ -143,11 +143,23 @@ let rec unfold_definition_and_simplify_eq (tm:term)
           let eq_h = implies_intro () in  // G, eq_h:x=e |- P
           rewrite eq_h; // G, eq_h:x=e |- P[e/x]
           clear ();     // G |- P[e/x]
-          visit (unfold_definition_and_simplify_eq tm)
+          visit (unfold_definition_and_simplify_eq' tm)
        end
 
+let unfold_definition_and_simplify_eq (tm:tactic term) 
+  : tactic unit 
+  = fun () -> unfold_definition_and_simplify_eq' (tm ()) ()
+
+let exact (t:tactic term) 
+  : tactic unit
+  = fun () -> FStar.Tactics.exact (t ())
+
+let apply_lemma (t:tactic term)
+  : tactic unit
+  = fun () -> FStar.Tactics.apply_lemma (t ())
+  
 ////////////////////////////////////////////////////////////////////////////////
-// End of tactic code 
+// End of tactic code
 ////////////////////////////////////////////////////////////////////////////////
 #reset-options "--use_tactics"
 
@@ -195,6 +207,7 @@ let partially_solved_using_smt =
                      pred_1 1)  //by another smt sub-goal
 
 assume val return_ten : unit -> Pure int (requires True) (ensures (fun x -> x == 10))
+
 let scanning_environment =
   let x = return_ten () in
   assert_by_tactic (seq (rewrite_equality (quote x))
@@ -203,12 +216,12 @@ let scanning_environment =
 
 assume val mul_comm : x:nat -> y:nat -> Tot (op_Multiply x y == op_Multiply y x)
 let test_exact (x:nat) (y:nat) =
-  assert_by_tactic (fun () -> exact (quote (mul_comm x y)))
+  assert_by_tactic (exact (quote (mul_comm x y)))
                    (op_Multiply x y == op_Multiply y x)
 
 
 let test_apply (x:nat) (y:nat) =
-  assert_by_tactic (fun () -> apply_lemma (quote lemma_mul_comm))
+  assert_by_tactic (apply_lemma (quote lemma_mul_comm))
                    (op_Multiply x y == op_Multiply y x)
 
 
